Unify lib/ with _dev

lib/Lib.Buffer.fst
@@ -555,9 +555,14 @@ let map_blocks_multi #t #a h0 bs nb inp output spec_f impl_f =
       (v i * v bs)
   )
 
-#reset-options "--z3rlimit 1000 --max_fuel 0 --max_ifuel 0 --z3cliopt smt.QI.EAGER_THRESHOLD=5"
+val div_mul_le: b:pos -> a:nat -> Lemma
+  ((a / b) * b <= a)
+let div_mul_le b a = ()
+
+#reset-options "--z3rlimit 500 --max_fuel 0 --max_ifuel 0"
 
 let map_blocks #t #a h0 len blocksize inp output spec_f spec_l impl_f impl_l =
+  div_mul_le (v blocksize) (v len);
   let nb = len /. blocksize in
   let rem = len %. blocksize in
   let blen = nb *! blocksize in
@@ -565,6 +570,7 @@ let map_blocks #t #a h0 len blocksize inp output spec_f spec_l impl_f impl_l =
   let ob = sub output 0ul blen in
   let il = sub inp blen rem in
   let ol = sub inp blen rem in
+  Math.Lemmas.lemma_div_mod (v len) (v blocksize);
   Math.Lemmas.multiple_division_lemma (v nb) (v blocksize);
   map_blocks_multi #t #a h0 blocksize nb ib ob spec_f impl_f;
   if rem >. 0ul then
